chore: integrate new PIR and pretty-printer
I still have to figure out how to setup the scopes/realizations correctly so simple-io wants to print the file

theories/PIR.v
@@ -1,5 +1,21 @@
-From Coq Require Import String.
+Require Import Coq.Strings.String.
+Require Import Coq.Init.Byte.
+Require Import Coq.Lists.List.
+Require Import Coq.ZArith.BinInt.
+Require Import Coq.Bool.BoolEq.
+Require Import Ascii.
+Require Import Eqdep.
+
+Set Implicit Arguments.
+
+Require Import Coq.Program.Basics.
+
+Import ListNotations.
 Local Open Scope string_scope.
+Local Open Scope Z_scope.
+
+(* Exports FunInd and used for tests later *)
+From QuickChick Require Import QuickChick.
 (* Restricted version of the AST from plutus-cert *)
 
 Inductive DefaultUni :=
@@ -7,6 +23,56 @@ Inductive DefaultUni :=
   | DefaultUniBool
   | DefaultUniUnit
 .
+
+(** Coq interpretation of plutus built-in types of base kind. If not of
+* base-kind (or not well-kinded), returns None.
+*)
+Definition uniType_option (x : DefaultUni) : option Set :=
+  match x with
+    | DefaultUniInteger    => Some Z
+    (* | DefaultUniByteString => Some (list byte) *)
+    (* | DefaultUniString => Some (list byte) UTF-8 encoded strings *)
+    | DefaultUniUnit => Some unit
+    (* | DefaultUniData => Some Data *)
+    (* | DefaultUniBLS12_381_G1_Element => Some Z *)
+    (* | DefaultUniBLS12_381_G2_Element => Some Z *)
+    (* | DefaultUniBLS12_381_MlResult => Some Z *)
+    | DefaultUniBool => Some bool
+
+    (* | DefaultUniApply DefaultUniProtoList t =>
+      match uniType_option t with
+        | None => None
+        | Some A => Some (list A)
+      end *)
+
+    (* | DefaultUniApply (DefaultUniApply DefaultUniProtoPair s) t =>
+      match uniType_option s, uniType_option t with
+      | Some A, Some B => Some (prod A B)
+      | _, _ => None
+      end
+
+    | DefaultUniApply _ _ => None
+    | DefaultUniProtoList => None
+    | DefaultUniProtoPair => None *)
+  end
+.
+Functional Scheme uniType_option_rect := Induction for uniType_option Sort Type.
+
+
+(** Coq interpretation of plutus built-in types of base kind. Used for constructing
+constants (See term.Constant). Types that are ill-kinded or do not have base kind are
+mapped to the empty type, ensuring that Constants of such type can be constructed.
+*)
+Definition uniType (x : DefaultUni) : Type :=
+  match uniType_option x with
+    | None => Empty_set
+    | Some ty => ty
+  end.
+
+(* Constants are coq values of the interpretation of some type in
+   DefaultUni *)
+Inductive constant :=
+  ValueOf : forall (T : DefaultUni), uniType T -> constant.
 
 Inductive DefaultFun :=
   | AddInteger
@@ -21,17 +87,34 @@ Inductive DefaultFun :=
   | LessThanEqualsInteger
 .
 
+Definition name := string.
+Definition tyname := string.
+Definition binderName := string.
+Definition binderTyname := string.
+
+(** kinds *)
+Inductive kind :=
+  | Kind_Base : kind
+  | Kind_Arrow : kind -> kind -> kind.
+
+(** Types *)
 Inductive ty :=
-  | Ty_Builtin : DefaultUni -> ty
+  (* | Ty_Var : tyname -> ty *)
   | Ty_Fun : ty -> ty -> ty
-  | UNDEFINED : string -> ty (* debug type *)
+  (* | Ty_IFix : ty -> ty -> ty *)
+  (* | Ty_Forall : binderTyname -> kind -> ty -> ty *)
+  | Ty_Builtin : DefaultUni -> ty
+  (* | Ty_Lam : binderTyname -> kind -> ty -> ty *)
+  (* | Ty_App : ty -> ty -> ty *)
+  (* | Ty_SOP : list (list ty) -> ty *)
+  | UNDEFINED : string -> ty
 .
 
 (* for now, we trust the string representing a value is correct *)
 Inductive term :=
-  | Var      : string -> term
-  | LamAbs   : string -> ty -> term -> term
-  | App      : term -> term -> term
+  | Var      : name -> term
+  | LamAbs   : binderName -> ty -> term -> term
+  | Apply    : term -> term -> term
   | Builtin  : DefaultFun -> term
-  | Constant : ty -> string -> term
+  | Constant : constant -> term
 .
