theories/Pretty.v
@@ -1,0 +1,263 @@
+From Coq Require Import String BinInt List.
+
+(* afaik Coq has no builtin string conversion methods
+for its primitive types so we import the ones from QuickChick *)
+From QuickChick Require Import Show.
+Import ShowFunctions.
+
+Import ListNotations.
+Local Open Scope string_scope.
+Local Open Scope Z_scope.
+
+From VTL Require Import PIR.
+
+Definition parens : string -> string :=
+  fun x => "(" ++ x ++ ")"
+.
+
+Definition brackets : string -> string :=
+  fun x => "[" ++ x ++ "]"
+.
+
+Definition braces : string -> string :=
+  fun x => "{" ++ x ++ "}"
+.
+
+Definition arrow : string -> string -> string :=
+  fun x y => x ++ " -> " ++ y
+.
+
+Definition sep (strs : list string) : string :=
+  string_concat (intersperse " " strs)
+.
+
+Definition sepr (sp : string) (strs : list string) : string :=
+  string_concat (intersperse sp strs)
+.
+
+(* TODO: improve span *)
+Definition sexp (op : string) (strs : list string) : string :=
+  "(" ++ op ++ " " (*++ newline*) ++ sep strs (*++ newline*) ++ ")"
+.
+
+Definition show_parens {A : Type} `{Show A} (x : A) : string :=
+  parens (show x)
+.
+
+Definition show_sep {A : Type} `{Show A} (xs : list A) : string :=
+  sep (map show xs)
+.
+
+Definition show_sexp {A : Type} `{Show A} (op : string) (xs : list A) : string :=
+  sexp op (map show xs)
+.
+
+(* Definition show_rec (rec : recursivity ) : string :=
+  match rec with
+  | NonRec => "nonrec"
+  | Rec    => "rec" 
+  end
+.
+
+#[global]
+Instance ShowRec : Show recursivity :=
+{|
+  show := show_rec
+|}.
+
+Definition show_strict (st : strictness) : string :=
+  match st with
+  | NonStrict => "nonstrict"
+  | Strict    => "strict" 
+  end
+.
+
+#[global]
+Instance ShowStrict : Show strictness :=
+{|
+  show := show_strict
+|}. *)
+
+
+Definition show_DefaultUni (U : DefaultUni) : string :=
+  match U with
+  | DefaultUniInteger => "integer"
+  (*| DefaultUniByteString => "bytestring" (*!*)
+  | DefaultUniString => "string" (*!*)*)
+  | DefaultUniUnit => "unit"
+  | DefaultUniBool => "bool"
+  (*| DefaultUniProtoList => "list" (* ! *)
+  | DefaultUniProtoPair => "pair" (* ! *)
+  | DefaultUniData => "data"
+  | DefaultUniBLS12_381_G1_Element => "bls12_381_G1_element"
+  | DefaultUniBLS12_381_G2_Element => "bls12_381_G2_element"
+  | DefaultUniBLS12_381_MlResult => "bls12_381_mlresult"
+
+  | DefaultUniApply U1 U2 =>
+      sep [show_DefaultUni U1 ; show_DefaultUni U2] (*!*)*)
+  end
+.
+
+#[global]
+Instance ShowDefaultUni : Show DefaultUni :=
+{|
+  show := show_DefaultUni
+|}.
+
+Definition show_Constant (cst : constant) : string :=
+  let val := match cst with
+  (* | ValueOf uni val => sep [show uni ; show val] end in 
+  (* is it possible to infer show for each unitype like the above? *) *)
+  | ValueOf DefaultUniInteger z => show_Z z
+  (* | ValueOf DefaultUniByteString bs => "NotImplemented:bs"
+  | ValueOf DefaultUniString str => "NotImplemented:str" *)
+  | ValueOf DefaultUniUnit u => "unit"
+  | ValueOf DefaultUniBool b => show_bool b end in
+  (* | ValueOf DefaultUniProtoList Us => "NotImplemented:protolist"
+  | ValueOf DefaultUniProtoPair Us => "NotImplemented:protopair"
+  | ValueOf DefaultUniData d => "NotImplemented:data"
+  | ValueOf DefaultUniBLS12_381_G1_Element z => show_Z z
+  | ValueOf DefaultUniBLS12_381_G2_Element z => show_Z z
+  | ValueOf DefaultUniBLS12_381_MlResult z => show_Z z
+  | ValueOf (DefaultUniApply U1 U2) U => "NotImplemented:apply" end in *)
+  sep [match cst with (ValueOf uni _) => show uni end ; val]
+.
+
+#[global]
+Instance ShowConstant : Show constant :=
+{|
+  show := show_Constant
+|}.
+
+(* TODO: copy all the other functions *)
+Definition show_DefaultFun (df : DefaultFun) : string :=
+  match df with
+  | AddInteger => "addInteger"
+  | SubtractInteger => "subtractInteger"
+  | MultiplyInteger => "multiplyInteger"
+  | DivideInteger => "divideInteger"
+  | QuotientInteger => "quotientInteger"
+  | RemainderInteger => "remainderInteger"
+  | ModInteger => "modInteger"
+  | EqualsInteger => "equalsInteger"
+  | LessThanInteger => "lessThanInteger"
+  | LessThanEqualsInteger => "lessThanEqualsInteger"
+  (* | _ => "UnknownDefaultFunction" *)
+  end
+.
+
+#[global]
+Instance ShowDefaultFun : Show DefaultFun :=
+{|
+  show := show_DefaultFun
+|}.
+
+(* Do we have datakinds? the plc pretty-printer does something with (type) here *)
+(*Fixpoint show_kind (k : kind) : string :=
+  match k with
+  | Kind_Base => "*"
+  | Kind_Arrow k1 k2 => sexp "fun" [show_kind k1 ; show_kind k2] (*!*) 
+  end
+.
+
+#[global]
+Instance ShowKind : Show kind :=
+{|
+  show := show_kind
+|}.*)
+
+Fixpoint show_ty (T : ty) : string :=
+  match T with
+  (*| Ty_Var tn => sep [tn] (*!*)*)
+  | Ty_Fun T1 T2 => sexp "fun" [show_ty T1 ; show_ty T2] (*!*)
+  (*| Ty_IFix T1 T2 => sexp "ifix" [show_ty T1 ; show_ty T2] (*!*)
+  | Ty_Forall btn k T => sexp "all" [btn ; show k ; show_ty T] (*!*)*)
+  | Ty_Builtin U => sexp "con" [show U]
+  | UNDEFINED err => braces err 
+  (*| Ty_Lam btn k T => sexp "lam" [btn ; show k ; show_ty T] (*!*)
+  | Ty_App T1 T2 => brackets (sep [show_ty T1 ; show_ty T2]) (*!*)*)
+  end
+.
+
+#[global]
+Instance ShowTy : Show ty :=
+{|
+  show := show_ty
+|}.
+
+(*Definition show_vdecl (vd : vdecl) : string :=
+  match vd with
+  | VarDecl bn T => sexp "vardecl" [bn ; show T]
+  end
+.
+
+#[global]
+Instance ShowVDecl : Show vdecl :=
+{|
+  show := show_vdecl
+|}.
+
+Definition show_tvdecl (tvd : tvdecl) : string :=
+  match tvd with
+  | TyVarDecl btn k => sexp "tyvardecl" [btn ; show_parens k]
+  end
+.
+
+#[global]
+Instance ShowTVDecl : Show tvdecl :=
+{|
+  show := show_tvdecl
+|}.
+
+Definition show_dtdecl (dtd : dtdecl) : string :=
+  match dtd with
+  | Datatype tvd tvds bn vds => sexp "datatype" [
+    show tvd ; show_sep tvds ;
+    bn ; show vds] (*!*)
+  end
+.
+
+#[global]
+Instance ShowDTDecl : Show dtdecl :=
+{|
+  show := show_dtdecl
+|}.*)
+
+Fixpoint show_term (t : term) : string :=
+  match t with
+  (* | Let rec bds t => sexp "let" [show_parens rec ;
+      sep (map show_binding bds) ; show_term t] *)
+  | Var x => sep [x]
+  (* | TyAbs bn k t => sexp "abs" [bn ; show k ; show_term t] *)
+  | LamAbs x T t => sexp "lam" [x  ; show T ; show_term t]
+  | Apply t1 t2 => brackets (sep [show_term t1 ; show_term t2])
+  | Constant cst => sexp "con" [show cst]
+  | Builtin def => sexp "builtin" [show def]
+  (* | TyInst t T => braces (sep [show_term t ; show T]) *)
+  (* | Error T => sexp "error" [show T] *)
+  (* | IWrap T1 T2 t => sexp "iwrap" [show T1 ; show T2 ; show_term t] *)
+  (* | Unwrap t => sexp "unwrap" [show_term t] *)
+  (* | Constr T n ts => sexp "consr" [show T ; show n ; sep (map show_term ts)] *)
+  (* | Case T t ts => sexp "case" [show T ; show_term t ; sep (map show_term ts)] *)
+  end
+
+(* with show_binding (b : binding) : string := 
+  match b with
+  | TermBind strc vdecl t => sexp "termbind" [
+      show strc ; show vdecl ; show_term t]
+  | TypeBind tvdecl T => sexp "typebind" [show tvdecl ; show T]
+  | DatatypeBind dtdecl => sexp "datatypebind" [show dtdecl]
+  end *)
+.
+
+#[global]
+Instance ShowTerm : Show term :=
+{|
+  show := show_term
+|}.
+
+Definition print_as_program (t : term) :=
+  sexp "program" ["1.1.0" ; show t]
+.
+
+(* Eval cbv in (print_as_program (LamAbs "x" (Ty_Builtin DefaultUniInteger) (Var "x"))). *)
