InvokePlutus.sh
@@ -1,0 +1,13 @@
+#! /bin/bash
+# Execute Printer.v and run the generated .pir file through the plutus compiler
+out=./output/test.pir
+plutus_path=../plutus/plutus
+make # there's an error in ./src/PlutusIR/Analysis/Size.v atm, luckily this does not interrupt the pipeline
+echo -e "\033[0;34mpir output:\033[0m"
+cat ${out}
+echo -e "\n"
+mkdir -p ${plutus_path}/input
+cp ${out} ${plutus_path}/input
+cd ${plutus_path}
+# assumes the plutus executable has been built in the past
+nix develop --command bash -c 'cabal exec -- plutus input/test.pir -o input/test.plc && echo -e "\n\033[0;33mplc output:\033[0m" && cat input/test.plc && echo -e "\n"'
