Makefile
@@ -719,7 +719,6 @@ clean::
 	$(HIDE)rm -f $(VFILES:.v=.glob)
 	$(HIDE)rm -f $(VFILES:.v=.tex)
 	$(HIDE)rm -f $(VFILES:.v=.g.tex)
-	$(HIDE)rm -f test.pir
 	$(HIDE)rm -f pretty-timed-success.ok
 	$(HIDE)rm -f META
 	$(HIDE)rm -rf html mlihtml
